in-flight entertainment is pretty bad. modified the footprints in the AEAD interface, using Pointer loc, added monotonicity, changed FileTransfer interface, verifying both the interfaces, and started to implement the FileTransfer app.

secure_api/aead/Crypto.AEAD.FileTransfer.fsti
@@ -1,106 +1,118 @@
 module Crypto.AEAD.FileTransfer
+
 open FStar.HyperStack.ST
+
 module AEAD = Crypto.AEAD.Main
-module HH = FStar.HyperHeap
 module I = Crypto.Indexing
 module P = FStar.Pointer
 
+module HH = FStar.HyperHeap
+module HS = FStar.HyperStack
+
+module Plain = Crypto.Plain
+
 noeq 
 type pre_id = {
-  reader_id : I.id;
-  writer_id : I.id
+  writer_id: I.id;
+  reader_id: I.id
 }
 
 type id = x:pre_id{x.reader_id =!= x.writer_id}
 
-let peer_id (x:id) : id = {
-  reader_id=x.writer_id;
-  writer_id=x.reader_id
+let peer_id (x:id) :id = {
+  writer_id = x.reader_id;
+  reader_id = x.writer_id
 }
 
-val my_nonce   : id -> nonce
-val my_region  : id -> mem -> GTot (option region)
+val my_nonce   :i:id -> (AEAD.nonce (i.writer_id))
+val my_region  :id -> HS.mem -> GTot (option HH.rid)  //AR: why is this an option?
 
-val peers_nonce: id -> nonce
-val peers_region: id -> mem -> GTot (option region)
+val peer_nonce :i:id -> (AEAD.nonce (i.reader_id))
+val peer_region:id -> HS.mem -> GTot (option HH.rid)
 
-noeq 
-type conn (i:id) : Type0
+val conn (i:id) :Type0  //adding noeq gives inconsistent qualifiers error
 
-//We need a max_plain_len from AEAD
+let plain_fragment (i:id) = l:AEAD.plainLen & Plain.plain i.writer_id l
 
-let plain_fragment (i:id) = l:Plain.plainLen{l < max_plain_len} & Plain.plain i.writer_id l
+//AR: how do we define this?
+val safeId: i:id -> GTot bool
+
+(** log, monotonicity **)
+
+val log_elt (i:id) :Type0
+
+val plain_of_log_elt: #i:_ -> log_elt i -> plain_fragment i
 
 //projection of the AEAD log
-val writer_log : i:_ -> conn i -> mem -> Seq.seq (plain_fragment i)
+val log: #i:_ -> c:conn i{safeId i} -> HS.mem -> GTot (Seq.seq (log_elt i))
 
-//Maybe useful to have a variant of this that allows you to snapshot
+//maybe useful to have a variant of this that allows you to snapshot
 //a sub-sequence of the log corresponding to a file that was sent
-val writer_log_contains : i:_ -> conn i -> Seq.seq (plain_fragment i) -> Type0
+val log_prefix: #i:_ -> c:conn i{safeId i} -> Seq.seq (log_elt i) -> Type0
 
-val witness_writer_log : i:_ -> conn i -> ST unit
-  (requires (fun _ -> True))
-  (ensures (fun h0 _ h1 -> h0 == h1 /\ writer_log_contains c (writer_log c h1)))
+val witness_log (#i:_) (c:conn i{safeId i})
+  :ST unit (requires (fun _       -> True))
+           (ensures  (fun h0 _ h1 -> h0 == h1 /\ log_prefix c (log c h0)))
 
-val recall_writer_log_contains: i:_ -> c:conn i -> s:Seq.seq (plain_fragment i) -> ST unit
-  (requires (fun _ -> write_log_contains c s))
-  (ensures (fun h0 _ h1 -> h0 == h1 /\ s `is_a_prefix_of` writer_log c h1))
+val recall_log (#i:_) (c:conn i{safeId i}) (s:Seq.seq (log_elt i))
+  :ST unit (requires (fun _      -> log_prefix c s))
+           (ensures (fun h0 _ h1 -> h0 == h1 /\ s `AEAD.is_prefix_of` (log c h0)))
   
-//Maybe it's useful to have some notion of append-only growth of witness_writer_log
+(* basically a conjunction of 2 AEAD invariants *)
+val conn_invariant: #i:_ -> conn i -> HS.mem -> Type0
 
-//val all_connnections :  we need this table to describe disjointness properties of all connections
+val conn_footprint: #i:_ -> conn i -> GTot P.loc
 
-val invariant : #i:_ -> conn i -> mem -> Type0 (* basically a conjunction of 2 AEAD invariants *)
+val lemma_frame_invariant_footprint (#i:_) (c:conn i) (h0 h1:HS.mem)
+   :Lemma (requires (conn_invariant c h0 /\
+                     P.unchanged (conn_footprint c) h0 h1))
+          (ensures  (conn_invariant c h1))
 
-val footprint : #i:_ -> conn i -> P.loc
+(* fragment a file into fragments that can be passed to AEAD *)
+val fragment_file (#i:id) (#len:nat) (file:Plain.plain i.writer_id len) :Seq.seq (plain_fragment i)
+val rebuild_file  (#i:id) (s:Seq.seq (plain_fragment i)) :(l:nat & Plain.plain i.writer_id l)
+val lemma_fragment_rebuild_inverse (#i:id) (#len:nat) (file:Plain.plain i.writer_id len)
+  :Lemma (rebuild_file (fragment_file file) == (| len, file |))
 
-val invariant_frame_unrelated: #i:_ -> c:conn i -> h0:mem -> h1:mem -> Lemma
-   (requires (invariant c h0 /\
-              loc_unchanged (footprint c) h0 h1)) //Q: how to express loc_unchanged? Does not seem to be in P
-   (requires (invariant c h1))
+val send (#i:_) (#len:nat) (c:conn i) (file:Plain.plain i.writer_id len)
+  :ST unit (requires (fun h0     -> conn_invariant c h0))
+           (ensures (fun h0 _ h1 -> P.modifies (conn_footprint c) h0 h1 /\
+                                 conn_invariant c h1                 /\
+                                 (safeId i ==>
+				  (let log0 = log c h0 in
+				   let log1 = log c h1 in
+				   log0 `AEAD.is_prefix_of` log1          /\
+				   AEAD.seq_map (plain_of_log_elt #i)
+				                (Seq.slice log1 (Seq.length log0)
+				                                (Seq.length log1)) ==
+	                           fragment_file file))))
 
-val fragment (#i:_) (#file_size_in_bytes:nat) (file:plain i file_size_in_bytes) : Seq.seq (plain_fragment i)
-val rebuild  (#i:_) (frags:Seq.seq (plain_fragment i)) : (l:nat & plain i l)
-val fragment_rebuild_inv (#i:_) (#file_size_in_bytes:nat) (file:plain i file_size_in_bytes) :
-    Lemma (rebuild (fragment file) == (| file_size_in_bytes, file |))
-
-val send : #i:_ -> #file_size_in_bytes:nat
-         -> c:conn i
-         -> file:plain i file_size_in_bytes
-         -> ST unit
-   (requires (fun h -> invariant c h /\
-                    global_inv h))
-   (ensures (fun h0 _ h1 -> 
-               modifies_loc (footprint c) h0 h1 /\
-               invariant c h1 /\
-               global_inv h1 /\
-               (safeId i ==> 
-                writer_log c h1 == Seq.append (write_log c h0) (fragment file))))
-
-
-val recv : #i:_
-         -> c:conn i
-         -> ST (option (file_size_in_bytes:nat & plain i file_size_in_bytes))
-   (requires (fun h -> invariant c h /\
-                    global_inv h))
-   (ensures (fun h0 f h1 -> 
-               modifies_loc (footprint c) h0 h1 /\
-               invariant c h1 /\
-               global_inv h1 /\
-               (safeId i ==> writer_log c h1 == writer_log c h0 /\
-                             (match f with 
-                              | None -> True
-                              | Some (| size, file |) -> 
-                                writer_log_contains c (fragment file)))))
+val recv (#i:_) (c:conn i)
+  :ST (option (len:nat & Plain.plain i.writer_id len))
+      (requires (fun h0      -> conn_invariant c h0))
+      (ensures  (fun h0 t h1 -> P.modifies (conn_footprint c) h0 h1 /\
+                             conn_invariant c h1                 /\
+                             (safeId i ==>
+			      (log c h1 == log c h0 /\
+                               (match t with 
+                                | None -> True
+                                | Some (| len, file |) ->
+				  (fragment_file file) `AEAD.is_subseq_of`
+				  (AEAD.seq_map (plain_of_log_elt #i) (log c h0)))))))
 
 
 
-let gen (i:id) (writer_region:rid) :
-  ST (conn i)
-     (requires (fun h -> safeId i ==> Some writer_region == nonce_to_region.[my_nonce i] /\
-                      global_inv h0))
-     (ensures (fun h0 c h1 -> modifies global_region h0 h1 /\
-                           MkConn?.w = writer_region /\
-                           global_inv h1 /\
-                           conn_inv c h))
+// let gen (i:id) (writer_region:rid) :
+//   ST (conn i)
+//      (requires (fun h -> safeId i ==> Some writer_region == nonce_to_region.[my_nonce i] /\
+//                       global_inv h0))
+//      (ensures (fun h0 c h1 -> modifies global_region h0 h1 /\
+//                            MkConn?.w = writer_region /\
+//                            global_inv h1 /\
+//                            conn_inv c h))
+
+
+
+
+//val all_connnections :we need this table to describe disjointness properties of all connections
 
