secure_api/aead/Crypto.AEAD.FileTransfer.fst
@@ -1,0 +1,54 @@
+module Crypto.AEAD.FileTransfer
+
+open FStar.HyperStack.ST
+
+module AEAD = Crypto.AEAD.Main
+module I = Crypto.Indexing
+module P = FStar.Pointer
+
+module HH = FStar.HyperHeap
+module HS = FStar.HyperStack
+
+module Plain = Crypto.Plain
+
+let my_nonce    i = magic ()
+let my_region   i = magic ()
+let peer_nonce  i = magic ()
+let peer_region i = magic ()
+
+private noeq type conn_aux (i:id) =
+  | C: writer:AEAD.aead_state i.writer_id I.Writer ->
+       reader:AEAD.aead_state i.reader_id I.Reader ->
+       conn_aux i
+
+let conn i = conn_aux i
+
+let safeId i = magic ()
+
+assume val lemma_safeId (i:id) :Lemma (requires (safeId i)) (ensures (AEAD.safeMac i.writer_id /\
+                                                                      AEAD.safeMac i.reader_id))
+				      [SMTPat (safeId i)]
+
+let log_elt (i:id)          = AEAD.entry i.writer_id
+let plain_of_log_elt #i elt = AEAD.plain_of_entry elt
+let log #i c h              = AEAD.log c.writer h
+let log_prefix #i c s       = AEAD.log_prefix c.writer s
+let witness_log #i c        = AEAD.witness_log c.writer
+let recall_log #i c s       = AEAD.recall_log c.writer s
+
+let conn_invariant #i c h =
+  let _ = () in
+  AEAD.aead_invariant c.writer h /\ AEAD.aead_invariant c.reader h
+
+(*
+ * footprint cannot be (write c.writer union read c.reader), else we can't prove framing
+ *)
+let conn_footprint #i c = P.loc_union (AEAD.write_footprint c.writer) (AEAD.write_footprint c.reader)
+
+let lemma_frame_invariant_footprint #i c h0 h1 =
+  AEAD.lemma_frame_invariant_footprint c.writer h0 h1;
+  AEAD.lemma_frame_invariant_footprint c.reader h0 h1
+
+let fragment_file #i #len file                  = magic ()
+let rebuild_file  #i s                          = magic ()
+let lemma_fragment_rebuild_inverse #i #len file = admit ()
